\section{Identities}


$$ \sum_{i=1}^{n} i = \frac{n(n+1)}{2}  $$

$$\sum_{i=1}^{n} i^{2} = \frac{n(n+1)(2n+1)}{6}  $$

$$\sum_{i=1}^{n} i^{3} = \frac{n^{2}(n+1)^{2}}{4} = \left(\sum_{i=1}^n i\right)^2$$

\subsection{Gemetric sequence}

\begin{equation}
  a, ar, ar^2, ar^3, \ldots ar^{n-1}
  \label{eq:Geometric sequence definition}
\end{equation}

$r$ should not be $0$

\subsubsection{Sum of the first $N$ terms}

\begin{equation}
  \sum_{k=0}^{n-1} ar^k =  a  \frac{1 - r^n}{1-r}
  \label{eq:Sum of the first N terms in a geometric sequence}
\end{equation}
